$$
A(x)B(x) \equiv 1 \pmod {x^n}\\
A(x)B'(x) \equiv 1 \pmod {x^{\small\left\lceil\frac{n}{2}\right\rceil}}\\
A(x)B'(x)-A(x)B(x) \equiv 0 \pmod {x^{\small\left\lceil\frac{n}{2}\right\rceil}}\\
B'(x)-B(x) \equiv 0 \pmod {x^{\small\left\lceil\frac{n}{2}\right\rceil}}\\
B'(x)^2-2B(x)B'(x)+B(x)^2 \equiv 0 \pmod {x^n}\\
A(x)(B'(x)^2-2B(x)B'(x)+B(x)^2) \equiv 0 \pmod {x^n}\\
A(x)B'(x)^2-2A(x)B(x)B'(x)+A(x)B(x)^2 \equiv 0 \pmod {x^n}\\
A(x)B'(x)^2-2B'(x)+B(x) \equiv 0 \pmod {x^n}\\
\boxed{B(x) \equiv B'(x)(2-A(x)B'(x)) \pmod {x^n}}\\


$$
